bitmap set

lib/Bitmap.i.dfy
@@ -2,10 +2,14 @@
 
 include "NativeTypes.s.dfy"
 include "Option.s.dfy"
+include "Marshalling/Native.s.dfy"
+include "BitsetLemmas.i.dfy"
 
 module Bitmap {
   import opened NativeTypes
   import opened Options
+  import Native
+  import BitsetLemmas
 
   type BitmapModel = seq<bool>
 
@@ -85,16 +89,24 @@ module Bitmap {
   class Bitmap {
     var bits: array<uint64>;
 
-    ghost var Contents: set<uint64>;
     ghost var Repr: set<object>;
 
-    static predicate {:opaque} BitBSet(word: uint64, b: nat)
+    static predicate BitBSet(word: uint64, b: uint64)
     requires b < 64
     {
-      && (word as bv64) & (1 << b) != 0
+      BitsetLemmas.in_set_uint64(b, word)
     }
 
-    static predicate BitsSetAtIB(bitsSeq: seq<uint64>, i: nat, b: nat)
+    lemma BitBSet0(b: uint64)
+    requires b < 64
+    ensures BitBSet(0, b) == false
+    {
+      BitsetLemmas.reveal_in_set_uint64();
+      BitsetLemmas.reveal_in_set();
+      BitsetLemmas.reveal_bit_and();
+    }
+
+    static predicate BitsSetAtIB(bitsSeq: seq<uint64>, i: nat, b: uint64)
     requires i < |bitsSeq|
     requires b < 64
     {
@@ -102,20 +114,14 @@ module Bitmap {
     }
 
     static predicate BitsSetAtC(bitsSeq: seq<uint64>, c: nat)
-    requires c / 64 < |bitsSeq|
+    requires c < 64 * |bitsSeq|
     {
-      && BitsSetAtIB(bitsSeq, c / 64, c % 64)
+      && BitsSetAtIB(bitsSeq, c / 64, (c % 64) as uint64)
     }
 
     static predicate ITimes64WithinUint64(i: nat)
     {
       && i * 64 < 0x1_0000_0000_0000_0000
-    }
-
-    static predicate {:opaque} BitsMatchesContents(bitsSeq: seq<uint64>, contents: set<uint64>)
-    {
-      && (forall c: nat | c < 0x1_0000_0000_0000_0000 && c / 64 < |bitsSeq| ::
-          c as uint64 in contents <==> BitsSetAtC(bitsSeq, c))
     }
 
     predicate ReprInv()
@@ -125,81 +131,63 @@ module Bitmap {
     }
 
     protected predicate Inv()
-    ensures Inv() ==> ReprInv()
+    ensures Inv() ==> this in this.Repr
     reads this, this.Repr
     {
       && ReprInv()
-
-      && BitsMatchesContents(bits[..], Contents)
     }
 
-    constructor (max: uint64)
-    requires max as nat < 0x1_0000_0000_0000_0000 / 2
-    ensures Contents == {}
-    ensures Inv()
+    static function {:opaque} IPrefix(bits: seq<uint64>, i: int) : (res : BitmapModel)
+    requires 0 <= i <= 64 * |bits|
+    ensures |res| == i
+    ensures forall j | 0 <= j < i :: res[j] == BitsSetAtC(bits, j)
     {
-      assert ((max / 64) + 1) * 64 > max;
-      bits := new [(max / 64) + 1] (_ => 0);
+      if i == 0 then [] else IPrefix(bits, i-1) + [BitsSetAtC(bits, i-1)]
+    }
 
+    protected function I() : BitmapModel
+    reads this, this.Repr
+    requires Inv()
+    {
+      IPrefix(bits[..], 64 * bits.Length)
+    }
+
+    constructor (len: uint64)
+    requires len as int < 0x1_0000_0000_0000_0000 / 2
+    requires len % 64 == 0
+    ensures Inv()
+    ensures I() == EmptyBitmap(len as int)
+    {
       new;
-
-      Contents := {};
+      bits := Native.Arrays.newArrayFill(len / 64, 0);
       Repr := { this, this.bits };
 
-      reveal_BitsMatchesContents();
-      reveal_BitBSet();
+      ghost var ghosty := true;
+      if ghosty {
+        forall j | 0 <= j < len
+        ensures I()[j] == EmptyBitmap(len as int)[j];
+        {
+          BitBSet0(j % 64);
+          reveal_IsSet();
+          //assert I()[j] == false;
+          assert !IsSet(EmptyBitmap(len as int), j as int);
+          //assert !EmptyBitmap(len as int)[j];
+          //assert EmptyBitmap(len as int)[j] == false;
+        }
+      }
     }
 
-    static function method {:opaque} SetBit(word: uint64, b: uint64) : uint64
+    static function method SetBit(word: uint64, b: uint64) : uint64
     requires b < 64
     {
-      (word as bv64 | (1 << b)) as uint64
+      BitsetLemmas.set_bit_to_1_uint64(word, b)
     }
-
-    // TODO ???
-    static lemma SetBitProperties(before: uint64, after: uint64, b: uint64)
-    requires b < 64
-    requires after == SetBit(before, b)
-    ensures BitBSet(after, b as nat)
-    ensures forall b': nat | b' != b as nat && b' < 64 :: BitBSet(after, b') <==> BitBSet(before, b')
-    {
-      assume false;
-    }
-
-    //== SetBitProperties attempts ==
-    //{
-    //  var beforeBV := before as bv64;
-    //  var afterBV := after as bv64;
-
-    //  forall ensures afterBV & (1 << b) != 0
-    //  {
-    //    reveal_SetBit();
-    //    assert before as nat < 0x1_0000_0000_0000_0000;
-    //    assert after as nat < 0x1_0000_0000_0000_0000;
-    //    assert after == (before as bv64 | (1 << b)) as uint64;
-    //    // TODO ???
-    //    assume afterBV == (beforeBV | (1 << b));
-    //    assume afterBV & (1 << b) != 0;
-    //  }
-    //  reveal_BitBSet();
-    //  assert BitBSet(after, b as nat);
-
-    //  forall b': nat | b' != b as nat && b' < 64
-    //  ensures BitBSet(after, b') <==> BitBSet(before, b')
-    //  {
-    //    assume false;
-    //    // TODO ???
-    //    if BitBSet(before, b') {
-    //    } else {
-    //    }
-    //  }
-    //}
 
     method Set(c: uint64)
-    requires c as nat / 64 < bits.Length
     requires Inv()
+    requires c as nat < Len(I())
     ensures Inv()
-    ensures Contents == old(Contents) + {c}
+    ensures I() == BitSet(old(I()), c as int)
     ensures this.Repr == old(this.Repr)
     modifies this, this.Repr
     {
@@ -207,30 +195,33 @@ module Bitmap {
       var b: uint64 := c % 64;
 
       this.bits[i] := SetBit(this.bits[i], b);
-      SetBitProperties(old(this.bits[i]), this.bits[i], b);
 
-      Contents := Contents + {c};
+      ghost var ghosty := true;
+      if ghosty {
+        reveal_BitSet();
+        reveal_IsSet();
 
-      forall c': nat | c' < 0x1_0000_0000_0000_0000 && c' / 64 < bits.Length
-      ensures c' as uint64 in Contents <==> BitsSetAtC(bits[..], c')
-      {
-        var i' := c' / 64;
-        var b' := c' % 64;
-        if i' == i as nat {
-          if b' == b as nat {
+        forall c' : int | 0 <= c' as int < 64 * this.bits.Length
+        ensures I()[c'] == BitSet(old(I()), c as int)[c']
+        {
+          var i' := c' / 64;
+          var b' := c' % 64;
+          if i' == i as nat {
+            if b' == b as nat {
+              BitsetLemmas.set_bit_to_1_self_uint64(old(this.bits[i]), b);
+              assert I()[c'] == BitSet(old(I()), c as int)[c'];
+            } else {
+              BitsetLemmas.set_bit_to_1_other_uint64(old(this.bits[i]), b, b' as uint64);
+              assert I()[c'] == BitSet(old(I()), c as int)[c'];
+            }
           } else {
-            reveal_BitsMatchesContents();
-            assert old(c' as uint64 in Contents) <==> BitsSetAtC(old(bits[..]), c'); // observe
+            assert I()[c'] == BitSet(old(I()), c as int)[c'];
           }
-        } else {
-          reveal_BitsMatchesContents();
-          assert old(c' as uint64 in Contents) <==> BitsSetAtC(old(bits[..]), c'); // observe
-          /* (doc) assert this.bits[c' / 64] == old(this.bits[c' / 64]); */
         }
       }
-      reveal_BitsMatchesContents();
     }
 
+/*
     static function method {:opaque} ClearBit(word: uint64, b: uint64) : uint64
     requires b < 64
     {
@@ -304,5 +295,6 @@ module Bitmap {
         reveal_BitBSet();
       }
     }
+    */
   }
 }
